renaming cdcl_W_ops; changing 2-WL functions

Weidenbach_Book/CDCL_Two_Watched_Literals_Implementation.thy
@@ -9,7 +9,7 @@ imports CDCL_Two_Watched_Literals DPLL_CDCL_W_Implementation
 begin
 
 type_synonym conc_twl_state =
-  "((nat, nat, nat list) marked_lit, nat literal list twl_clause list, nat, nat literal list)
+  "((nat, nat, nat literal list) marked_lit, nat literal list twl_clause list, nat, nat literal list)
     twl_state"
 
 fun convert :: "('a, 'b, 'c list) marked_lit \<Rightarrow> ('a, 'b, 'c multiset) marked_lit"  where
@@ -30,220 +30,59 @@ abbreviation convert_clss :: "'v literal list twl_clause list \<Rightarrow> 'v c
   where
 "convert_clss S \<equiv> mset (map raw_clause_l S)"
 
-fun raw_state_of_conc :: "conc_twl_state \<Rightarrow> (nat, nat, nat multiset) twl_state_abs" where
+fun raw_state_of_conc :: "conc_twl_state \<Rightarrow> (nat, nat, nat clause) twl_state_abs" where
 "raw_state_of_conc (TWL_State M N U k C) =
   TWL_State (convert_tr M) (convert_clss N) (convert_clss U) k (map_option mset C)"
 
+lemma
+  "raw_state_of_conc (tl_trail S) = tl_trail (raw_state_of_conc S)"
+  unfolding tl_trail_def by (induction S) (auto simp: map_tl)
 
-subsection \<open>Abstract Implementation\<close>
+definition watch_nat :: "conc_twl_state \<Rightarrow> nat literal list \<Rightarrow> nat literal list twl_clause" where
+  "watch_nat S C =
+   (let
+      C' = remdups C;
+      negation_not_assigned = filter (\<lambda>L. -L \<notin> lits_of (trail S)) C';
+      negation_assigned_sorted_by_trail = filter (\<lambda>L. L \<in> set C) (map (\<lambda>L. -lit_of L) (trail S));
+      W = take 2 (negation_not_assigned @ negation_assigned_sorted_by_trail);
+      UW = foldl (\<lambda>a l. remove1 l a) C W
+    in TWL_Clause W UW)"
 
-text \<open>We define here a locale serving as proxy between the abstract transition defined using
-  multiset and a more concrete version using a representation that can be converted to lists.
-  \<close>
+definition
+  rewatch_nat ::
+  "(nat, nat, nat literal list) marked_lit \<Rightarrow> conc_twl_state \<Rightarrow>
+    nat literal list twl_clause \<Rightarrow> nat literal list twl_clause"
+where
+  "rewatch_nat L S C =
+   (if - lit_of L \<in> set (watched C) then
+      case filter (\<lambda>L'. L' \<notin> set (watched C) \<and> - L' \<notin> lits_of (L # trail S))
+          (unwatched C) of
+        [] \<Rightarrow> C
+      | L' # _ \<Rightarrow>
+        TWL_Clause (L' # remove1 (- lit_of L) (watched C)) 
+          (- lit_of L # remove1 L' (unwatched C))
+    else
+      C)"
 
-subsubsection \<open>An Extend State\<close>
+definition raw_candidates_conflict :: "conc_twl_state \<Rightarrow> nat literal list list" where
+  "raw_candidates_conflict S =
+    map (\<lambda>T. case T of TWL_Clause W UW \<Rightarrow> W @ UW)
+       (filter (\<lambda>C. set (watched C) \<subseteq> (uminus ` lits_of (trail S))) 
+       (init_clss S @ learned_clss S))"
 
-text \<open>The more concrete state has some way to find candidates. This is abstracted, since it can be
-  integrated to the data-structure (see 2-watched literals) \<close>
-locale conc_state\<^sub>W_with_candidates =
-  state\<^sub>W trail init_clss learned_clss backtrack_lvl conflicting cons_trail tl_trail add_init_cls
-   add_learned_cls remove_cls update_backtrack_lvl update_conflicting init_state
-   restart_state
-  for
-    trail :: "'st \<Rightarrow> ('v, nat, 'v clause) marked_lits" and
-    init_clss :: "'st \<Rightarrow> 'v clauses" and
-    learned_clss :: "'st \<Rightarrow> 'v clauses" and
-    backtrack_lvl :: "'st \<Rightarrow> nat" and
-    conflicting :: "'st \<Rightarrow>'v clause option" and
-
-    cons_trail :: "('v, nat, 'v clause) marked_lit \<Rightarrow> 'st \<Rightarrow> 'st" and
-    tl_trail :: "'st \<Rightarrow>'st" and
-    add_init_cls :: "'v clause \<Rightarrow> 'st \<Rightarrow> 'st" and
-    add_learned_cls :: "'v clause \<Rightarrow> 'st \<Rightarrow> 'st" and
-    remove_cls :: "'v clause \<Rightarrow> 'st \<Rightarrow> 'st" and
-    update_backtrack_lvl :: "nat \<Rightarrow> 'st \<Rightarrow> 'st" and
-    update_conflicting :: "'v clause option \<Rightarrow> 'st \<Rightarrow> 'st" and
-
-    init_state :: "'v clauses \<Rightarrow> 'st" and
-    restart_state :: "'st \<Rightarrow> 'st" +
-  fixes
-    raw_trail :: "'conc_st \<Rightarrow> 'trail" and
-    raw_init_clss :: "'conc_st \<Rightarrow> 'clss" and
-    raw_learned_clss :: "'conc_st \<Rightarrow> 'clss" and
-    raw_backtrack_lvl :: "'conc_st \<Rightarrow> nat" and
-    raw_conflicting :: "'conc_st \<Rightarrow> 'cls option" and
-
-    raw_cons_trail :: "('v, nat, 'cls) marked_lit \<Rightarrow> 'conc_st \<Rightarrow> 'conc_st" and
-    raw_tl_trail :: "'conc_st \<Rightarrow>'conc_st" and
-    raw_add_init_cls :: "'cls \<Rightarrow> 'conc_st \<Rightarrow> 'conc_st" and
-    raw_add_learned_cls :: "'cls \<Rightarrow> 'conc_st \<Rightarrow> 'conc_st" and
-    raw_remove_cls :: "'cls \<Rightarrow> 'conc_st \<Rightarrow> 'conc_st" and
-    raw_update_backtrack_lvl :: "nat \<Rightarrow> 'conc_st \<Rightarrow> 'conc_st" and
-    raw_update_conflicting :: "'cls option \<Rightarrow> 'conc_st \<Rightarrow> 'conc_st" and
-
-    raw_init_state :: "'clss \<Rightarrow> 'conc_st" and
-    raw_restart_state :: "'conc_st \<Rightarrow> 'conc_st" and
-    get_propagate_candidates :: "'conc_st \<Rightarrow> ('v literal \<times> 'cls) list" and
-    get_conflict_candidates :: "'conc_st \<Rightarrow> 'cls list" and
-    get_not_decided :: "'conc_st \<Rightarrow> 'v literal option" and
-
-    st_of_raw :: "'conc_st \<Rightarrow> 'st" and
-    cls_of_raw_cls :: "'cls \<Rightarrow> 'v clause" and
-    clss_of_raw_clss :: "'clss \<Rightarrow> 'v clause list" and
-    raw_cls_union :: "'cls \<Rightarrow> 'cls \<Rightarrow> 'cls" and
-    remdups_raw_cls :: "'cls \<Rightarrow> 'cls" and
-    marked_lit_of_raw :: "('v, nat, 'cls) marked_lit \<Rightarrow> ('v, nat, 'v clause) marked_lit" and
-    maximum_level :: "'cls \<Rightarrow> 'conc_st \<Rightarrow> nat" and
-    raw_hd_trail :: "'conc_st \<Rightarrow> ('v, nat, 'cls) marked_lit" and
-    remove :: "'v literal \<Rightarrow> 'cls \<Rightarrow> 'cls"
-
-  assumes
-    (* Mapping from 'cons_st to 'st *)
-    raw_cons_trail[simp]:
-      "\<And>L S. st_of_raw (raw_cons_trail L S) = cons_trail (marked_lit_of_raw L) (st_of_raw S)" and
-    raw_tl_trail[simp]:
-      "\<And>S. st_of_raw (raw_tl_trail S) = tl_trail (st_of_raw S)" and
-    raw_add_init_cls[simp]:
-      "\<And>C S. st_of_raw (raw_add_init_cls C S) = add_init_cls (cls_of_raw_cls C) (st_of_raw S)" and
-    raw_add_learned_cls[simp]:
-      "\<And>C S.
-        st_of_raw (raw_add_learned_cls C S) = add_learned_cls (cls_of_raw_cls C) (st_of_raw S)" and
-    raw_backtrack_lvl:
-      "raw_backtrack_lvl S = backtrack_lvl (st_of_raw S)" and
-    raw_update_backtrack_lvl[simp]:
-      "\<And>k S. st_of_raw (raw_update_backtrack_lvl k S) = update_backtrack_lvl k (st_of_raw S)" and
-    raw_update_conflicting[simp]:
-      "\<And>(C::'cls option) S. st_of_raw (raw_update_conflicting C S) =
-         update_conflicting (map_option cls_of_raw_cls C) (st_of_raw S)" and
-    raw_init_state:
-      "\<And>N. st_of_raw (raw_init_state N) = init_state (mset (clss_of_raw_clss N))" and
-    cls_of_raw_cls_raw_cls_union[simp]:
-      "cls_of_raw_cls (raw_cls_union a b) = cls_of_raw_cls a #\<union> cls_of_raw_cls b" and
-    cls_of_raw_cls_remdups_raw_cls[simp]:
-      "cls_of_raw_cls (remdups_raw_cls a) = remdups_mset (cls_of_raw_cls a)" and
-    conflicting_raw_conflicting:
-      "conflicting (st_of_raw S) = map_option cls_of_raw_cls (raw_conflicting S)" and
-    marked_lit_of_raw[simp]:
-      "\<And>L C. marked_lit_of_raw (Propagated L C) = Propagated L (cls_of_raw_cls C)"
-      "\<And>L i. marked_lit_of_raw (Marked L i) = Marked L i"
-      and
-    maximum_level[simp]:
-      "maximum_level C S = get_maximum_level (trail (st_of_raw S)) (cls_of_raw_cls C)" and
-    raw_hd_trail:
-      "\<And>S. trail (st_of_raw S) \<noteq> [] \<Longrightarrow>
-        marked_lit_of_raw (raw_hd_trail S) = hd (trail (st_of_raw S))" and
-    remove[simp]:
-      "cls_of_raw_cls (remove L C) = cls_of_raw_cls C - {#L#}" and
-
-    (* getting answers from the data-structure *)
-    get_conflict_candidates_empty:
-      "\<And>S. get_conflict_candidates S = [] \<longleftrightarrow>
-        (\<forall>D \<in># clauses (st_of_raw S). \<not> trail (st_of_raw S) \<Turnstile>as CNot D)" and
-    get_conflict_candidates_in_clauses:
-      "\<And>S. \<forall>C \<in> set (get_conflict_candidates S). cls_of_raw_cls C \<in># clauses (st_of_raw S) \<and>
-        trail (st_of_raw S) \<Turnstile>as CNot (cls_of_raw_cls C)" and
-    get_propagate_candidates_lit_in_cls:
-      "\<And>S. \<forall>(L, C) \<in> set (get_propagate_candidates S). undefined_lit (trail (st_of_raw S)) L \<and>
-        cls_of_raw_cls C \<in># clauses (st_of_raw S)
-        \<and> trail (st_of_raw S) \<Turnstile>as CNot (cls_of_raw_cls C - {#L#}) \<and> L \<in># cls_of_raw_cls C" and
-    get_propagate_candidates_empty:
-      "\<And>S. get_propagate_candidates S = [] \<longleftrightarrow>
-        \<not>(\<exists>C L. undefined_lit (trail (st_of_raw S)) L \<and> C + {#L#} \<in># clauses (st_of_raw S) \<and>
-          trail (st_of_raw S) \<Turnstile>as CNot C)" and
-    get_not_decided_Some:
-      "\<And>S L. get_not_decided S = Some L \<Longrightarrow>
-         undefined_lit (trail (st_of_raw S)) L \<and> atm_of L \<in> atms_of_msu (init_clss (st_of_raw S))"
-      and
-    get_not_decided_None:
-      "\<And>S. get_not_decided S = None \<Longrightarrow>
-         \<not>(\<exists>L. undefined_lit (trail (st_of_raw S)) L \<and>
-         atm_of L \<in> atms_of_msu (init_clss (st_of_raw S)))"
-
-subsubsection \<open>Lowering from Transitions to Functions\<close>
-locale
-  cdcl\<^sub>W_cands =
-   conc_state\<^sub>W_with_candidates trail init_clss learned_clss backtrack_lvl conflicting cons_trail
-   tl_trail
-   add_init_cls add_learned_cls remove_cls update_backtrack_lvl update_conflicting init_state
-   restart_state
-
-   raw_trail raw_init_clss raw_learned_clss raw_backtrack_lvl raw_conflicting raw_cons_trail
-   raw_tl_trail
-   raw_add_init_cls raw_add_learned_cls raw_remove_cls raw_update_backtrack_lvl
-   raw_update_conflicting raw_init_state
-   raw_restart_state
-
-   get_propagate_candidates get_conflict_candidates get_not_decided st_of_raw
-   cls_of_raw_cls clss_of_raw_clss
-   raw_cls_union remdups_raw_cls marked_lit_of_raw
-   maximum_level raw_hd_trail remove
-  for
-    trail :: "'st \<Rightarrow> ('v::linorder, nat, 'v::linorder clause) marked_lits" and
-    init_clss :: "'st \<Rightarrow> 'v clauses" and
-    learned_clss :: "'st \<Rightarrow> 'v clauses" and
-    backtrack_lvl :: "'st \<Rightarrow> nat" and
-    conflicting :: "'st \<Rightarrow>'v clause option" and
-
-    cons_trail :: "('v, nat, 'v clause) marked_lit \<Rightarrow> 'st \<Rightarrow> 'st" and
-    tl_trail :: "'st \<Rightarrow> 'st" and
-    add_init_cls :: "'v clause \<Rightarrow> 'st \<Rightarrow> 'st" and
-    add_learned_cls :: "'v clause \<Rightarrow> 'st \<Rightarrow> 'st" and
-    remove_cls :: "'v clause \<Rightarrow> 'st \<Rightarrow> 'st" and
-    update_backtrack_lvl :: "nat \<Rightarrow> 'st \<Rightarrow> 'st" and
-    update_conflicting :: "'v clause option \<Rightarrow> 'st \<Rightarrow> 'st" and
-
-    init_state :: "'v clauses \<Rightarrow> 'st" and
-    restart_state :: "'st \<Rightarrow> 'st" and
-
-    raw_trail :: "'conc_st \<Rightarrow> 'trail" and
-    raw_init_clss :: "'conc_st \<Rightarrow> 'clss" and
-    raw_learned_clss :: "'conc_st \<Rightarrow> 'clss" and
-    raw_backtrack_lvl :: "'conc_st \<Rightarrow> nat" and
-    raw_conflicting :: "'conc_st \<Rightarrow> 'cls option" and
-
-    raw_cons_trail :: "('v, nat, 'cls) marked_lit \<Rightarrow> 'conc_st \<Rightarrow> 'conc_st" and
-    raw_tl_trail :: "'conc_st \<Rightarrow>'conc_st" and
-    raw_add_init_cls :: "'cls \<Rightarrow> 'conc_st \<Rightarrow> 'conc_st" and
-    raw_add_learned_cls :: "'cls \<Rightarrow> 'conc_st \<Rightarrow> 'conc_st" and
-    raw_remove_cls :: "'cls \<Rightarrow> 'conc_st \<Rightarrow> 'conc_st" and
-    raw_update_backtrack_lvl :: "nat \<Rightarrow> 'conc_st \<Rightarrow> 'conc_st" and
-    raw_update_conflicting :: "'cls option \<Rightarrow> 'conc_st \<Rightarrow> 'conc_st" and
-
-    raw_init_state :: "'clss \<Rightarrow> 'conc_st" and
-    raw_restart_state :: "'conc_st \<Rightarrow> 'conc_st" and
-    get_propagate_candidates :: "'conc_st \<Rightarrow> ('v literal \<times> 'cls) list" and
-    get_conflict_candidates :: "'conc_st \<Rightarrow> 'cls list" and
-    get_not_decided :: "'conc_st \<Rightarrow> 'v literal option" and
-
-    st_of_raw :: "'conc_st \<Rightarrow> 'st" and
-    cls_of_raw_cls :: "'cls \<Rightarrow> 'v clause" and
-    clss_of_raw_clss :: "'clss \<Rightarrow> 'v clause list" and
-    raw_cls_union :: "'cls \<Rightarrow> 'cls \<Rightarrow> 'cls" and
-    remdups_raw_cls :: "'cls \<Rightarrow> 'cls" and
-    marked_lit_of_raw :: "('v, nat, 'cls) marked_lit \<Rightarrow> ('v, nat, 'v clause) marked_lit" and
-    maximum_level :: "'cls \<Rightarrow> 'conc_st \<Rightarrow> nat" and
-    raw_hd_trail :: "'conc_st \<Rightarrow> ('v, nat, 'cls) marked_lit" and
-    remove :: "'v literal \<Rightarrow> 'cls \<Rightarrow> 'cls"
-begin
-
-interpretation cdcl\<^sub>W_termination trail init_clss learned_clss backtrack_lvl conflicting cons_trail
-  tl_trail add_init_cls add_learned_cls remove_cls update_backtrack_lvl update_conflicting
-  init_state restart_state
- by unfold_locales
-
-paragraph \<open>The transitions\<close>
-definition do_conflict_step :: "'conc_st \<Rightarrow> 'conc_st option" where
+definition do_conflict_step :: "conc_twl_state \<Rightarrow> conc_twl_state option" where
 "do_conflict_step S =
-  (case raw_conflicting S of
+  (case conflicting S of
     Some _ \<Rightarrow> None
   | None \<Rightarrow>
-      (case get_conflict_candidates S of
+      (case raw_candidates_conflict S of
         [] \<Rightarrow> None
-      | a # _ \<Rightarrow> Some (raw_update_conflicting (Some a) S)))"
-
+      | a # _ \<Rightarrow> Some (update_conflicting (Some a) S)))"
+term twl.cons_trail 
+(* 
 lemma do_conflict_step_Some:
   assumes conf: "do_conflict_step S = Some T"
-  shows "conflict (st_of_raw S) (st_of_raw T)"
+  shows "twl.cdcl\<^sub>W_twl.conflict (st_of_raw S) (st_of_raw T)"
 proof (cases "raw_conflicting S")
   case Some
   then show ?thesis using conf unfolding do_conflict_step_def by simp
@@ -443,320 +282,5 @@ definition do_bj_step :: "'conc_st \<Rightarrow> 'conc_st option" where
     (case do_resolve_step S of
       Some T \<Rightarrow> Some T
     | None \<Rightarrow> do_backtrack_step S))"
-end
-
-subsection \<open>Implementation as list\<close>
-type_synonym 'a cdcl\<^sub>W_mark = "'a clause"
-type_synonym cdcl\<^sub>W_marked_level = nat
-
-type_synonym 'v cdcl\<^sub>W_marked_lit = "('v, cdcl\<^sub>W_marked_level, 'v cdcl\<^sub>W_mark) marked_lit"
-type_synonym 'v cdcl\<^sub>W_marked_lits = "('v, cdcl\<^sub>W_marked_level, 'v cdcl\<^sub>W_mark) marked_lits"
-type_synonym 'v cdcl\<^sub>W_state =
-  "'v cdcl\<^sub>W_marked_lits \<times> 'v clauses \<times> 'v clauses \<times> nat \<times> 'v clause option"
-
-abbreviation trail :: "'a \<times> 'b \<times> 'c \<times> 'd \<times> 'e \<Rightarrow> 'a" where
-"trail \<equiv> (\<lambda>(M, _). M)"
-
-abbreviation cons_trail :: "'a \<Rightarrow> 'a list \<times> 'b \<times> 'c \<times> 'd \<times> 'e \<Rightarrow> 'a list \<times> 'b \<times> 'c \<times> 'd \<times> 'e"
-  where
-"cons_trail \<equiv> (\<lambda>L (M, S). (L#M, S))"
-
-abbreviation tl_trail :: "'a list \<times> 'b \<times> 'c \<times> 'd \<times> 'e \<Rightarrow> 'a list \<times> 'b \<times> 'c \<times> 'd \<times> 'e" where
-"tl_trail \<equiv> (\<lambda>(M, S). (tl M, S))"
-
-abbreviation clauses :: "'a \<times> 'b \<times> 'c \<times> 'd \<times> 'e \<Rightarrow> 'b" where
-"clauses \<equiv> \<lambda>(M, N, _). N"
-
-abbreviation learned_clss :: "'a \<times> 'b \<times> 'c \<times> 'd \<times> 'e \<Rightarrow> 'c" where
-"learned_clss \<equiv> \<lambda>(M, N, U, _). U"
-
-abbreviation backtrack_lvl :: "'a \<times> 'b \<times> 'c \<times> 'd \<times> 'e \<Rightarrow> 'd" where
-"backtrack_lvl \<equiv> \<lambda>(M, N, U, k, _). k"
-
-abbreviation update_backtrack_lvl :: "'d \<Rightarrow> 'a \<times> 'b \<times> 'c \<times> 'd \<times> 'e \<Rightarrow> 'a \<times> 'b \<times> 'c \<times> 'd \<times> 'e"
-  where
-"update_backtrack_lvl \<equiv> \<lambda>k (M, N, U, _, S).  (M, N, U, k, S)"
-
-abbreviation conflicting :: "'a \<times> 'b \<times> 'c \<times> 'd \<times> 'e \<Rightarrow> 'e" where
-"conflicting \<equiv> \<lambda>(M, N, U, k, D). D"
-
-abbreviation update_conflicting :: "'e \<Rightarrow> 'a \<times> 'b \<times> 'c \<times> 'd \<times> 'e \<Rightarrow> 'a \<times> 'b \<times> 'c \<times> 'd \<times> 'e"
-  where
-"update_conflicting \<equiv> \<lambda>C (M, N, U, k, _).  (M, N, U, k, C)"
-
-abbreviation "S0_cdcl\<^sub>W N \<equiv> (([], N, {#}, 0, None):: 'v cdcl\<^sub>W_state)"
-
-abbreviation add_learned_cls where
-"add_learned_cls \<equiv> \<lambda>C (M, N, U, S). (M, N, {#C#} + U, S)"
-
-abbreviation remove_cls where
-"remove_cls \<equiv> \<lambda>C (M, N, U, S). (M, remove_mset C N, remove_mset C U, S)"
-
-lemma convert_Propagated[elim!]:
-  "convert z = Propagated L C \<Longrightarrow> (\<exists>C'. z = Propagated L C' \<and> C = mset C')"
-  by (cases z) auto
-
-type_synonym cdcl\<^sub>W_state_inv_st = "(nat, nat, nat clause) marked_lit list \<times>
-  nat literal list list \<times> nat literal list list \<times> nat \<times> nat literal list option"
-
-fun maximum_level_code:: "'a literal list \<Rightarrow> ('a, nat, 'a literal list) marked_lit list \<Rightarrow> nat"
-  where
-"maximum_level_code [] _ = 0" |
-"maximum_level_code (L # Ls) M = max (get_level M L) (maximum_level_code Ls M)"
-
-lemma maximum_level_code_eq_get_maximum_level[code, simp]:
-  "maximum_level_code D M = get_maximum_level M (mset D)"
-  by (induction D) (auto simp add: get_maximum_level_plus)
-
-lemma get_rev_level_convert_tr:
-  "get_rev_level (convert_tr M) n = get_rev_level M n"
-  by (induction M arbitrary: n rule: marked_lit_list_induct) auto
-
-lemma get_level_convert_tr:
-  "get_level (convert_tr M) = get_level M"
-  by (simp add: get_rev_level_convert_tr rev_map)
-
-lemma get_maximum_level_convert_tr[simp]:
-  "get_maximum_level (convert_tr M) (mset D) = get_maximum_level M (mset D)"
-  by (induction D) (simp_all add: get_maximum_level_plus get_level_convert_tr)
-
-interpretation cdcl\<^sub>W: state\<^sub>W
-  trail
-  "\<lambda>S. mset (clauses S)"
-  "\<lambda>S. mset (learned_clss S)"
-  backtrack_lvl conflicting
-  "\<lambda>L (M, S). (L # M, S)"
-  "\<lambda>(M, S). (tl M, S)"
-  "\<lambda>C (M, N, S). (M, C # N, S)"
-  "\<lambda>C (M, N, U, S). (M, N, C # U, S)"
-  "\<lambda>C (M, N, U, S). (M, removeAll C N, removeAll C U, S)"
-  "\<lambda>(k::nat) (M, N, U, _, D). (M, N, U, k, D)"
-  "\<lambda>D (M, N, U, k, _). (M, N, U, k, D)"
-  "\<lambda>N. ([], sorted_list_of_multiset N, [], 0, None)"
-  "\<lambda>(_, N, U, _). ([], N, U, 0, None)"
-  by unfold_locales (auto simp: add.commute)
-
-fun find_conflict where
-"find_conflict M [] = None" |
-"find_conflict M (N # Ns) = (if (\<forall>c \<in> set N. -c \<in> lits_of M) then Some N else find_conflict M Ns)"
-
-lemma find_conflict_Some:
-  "find_conflict M Ns = Some N \<Longrightarrow> N \<in> set Ns \<and> M \<Turnstile>as CNot (mset N)"
-  by (induction Ns rule: find_conflict.induct)
-     (auto split: split_if_asm)
-
-lemma find_conflict_None:
-  "find_conflict M Ns = None \<longleftrightarrow> (\<forall>N \<in> set Ns. \<not>M \<Turnstile>as CNot (mset N))"
-  by (induction Ns) auto
-
-lemma find_conflict_sorted_list_of_multiset_None:
-  "find_conflict M (map sorted_list_of_multiset Ns) = None \<longleftrightarrow> (\<forall>N \<in> set Ns. \<not>M \<Turnstile>as CNot N)"
-  by (simp add: find_conflict_None)
-
-lemma find_conflict_sorted_list_of_multiset_2_None:
-  "find_conflict M (map sorted_list_of_multiset Ns @ map sorted_list_of_multiset Ns') = None
-  \<longleftrightarrow> (\<forall>N \<in> set Ns \<union> set Ns'. \<not>M \<Turnstile>as CNot N)"
-  by (metis find_conflict_sorted_list_of_multiset_None map_append set_append)
-
-declare cdcl\<^sub>W.state_simp[simp del] cdcl\<^sub>W.clauses_def[simp add]
-
-lemma mset_map_mset_removeAll_remove_mset:
-  "C \<in> set N \<Longrightarrow> distinct (map mset N) \<Longrightarrow>
-  mset (map mset (removeAll C N)) = remove_mset (mset C) (mset (map mset N))"
-proof (induction N)
-  case Nil
-  then show ?case by simp
-next
-  case (Cons a N) note IH = this(1) and C = this(2) and dist = this(3)
-  have dist': "distinct (map mset N)"
-    using dist by auto
-  have H: "mset (map mset (removeAll C N)) = remove_mset (mset C) (mset (map mset N))"
-    by (metis C IH count_mset_0 diff_zero dist distinct.simps(2) list.simps(9) removeAll_id
-      replicate_mset_0 set_ConsD)
-  have rall: "mset (map mset (removeAll C (a # N))) =
-     (if C = a then {#} else {#mset a#}) + mset (map mset (removeAll C N))"
-     by (auto simp: ac_simps)
-  have rmset: "remove_mset (mset C) (mset (map mset (a # N))) =
-     (if mset C = mset a then {#} else {#mset a#}) + remove_mset (mset C) (mset (map mset N))"
-    proof -
-      { assume a1: "mset C \<noteq> mset a"
-        then have "remove_mset (mset C) (mset (map mset (a # N))) - {#mset a#} + {#mset a#}
-          = remove_mset (mset C) (mset (map mset (a # N))) - {#}"
-          by simp (* 3 ms *)
-        then have ?thesis
-          using a1 by (simp_all add: Multiset.diff_right_commute add.commute)}
-      then show ?thesis
-        by (cases "mset C \<noteq> mset a") (auto simp: ac_simps)
-    qed
-  have "C \<noteq> a \<longrightarrow> mset C \<noteq> mset a"
-    by (metis C dist distinct.simps(2) image_eqI list.simps(9) set_ConsD set_map)
-  then show ?case
-    unfolding rall rmset H by simp
-qed
-
-interpretation cdcl\<^sub>W':  state\<^sub>W
-  trail
-  clauses
-  learned_clss
-  backtrack_lvl conflicting
-  "\<lambda>L (M, S). (L # M, S)"
-  "\<lambda>(M, S). (tl M, S)"
-  "\<lambda>C (M, N, S). (M, {#C#} + N, S)"
-  "\<lambda>C (M, N, U, S). (M, N, {#C#} + U, S)"
-  "\<lambda>C (M, N, U, S). (M, remove_mset C N, remove_mset C U, S)"
-  "\<lambda>k (M, N, (U::nat clauses), _, D). (M, N, U, k, D)"
-  "\<lambda>D (M, N, U, k, _). (M, N, U, k, D)"
-  "\<lambda>N. ([], N, {#}, 0, None)"
-  "\<lambda>(_, N, U, _). ([], N, U, 0, None)"
-  by unfold_locales auto
-
-fun union_mset_list :: "'a list \<Rightarrow> 'a list \<Rightarrow> 'a list" where
-"union_mset_list [] l = l" |
-"union_mset_list (a # l) l' = a # union_mset_list l (remove1 a l')"
-
-lemma mset_union_mset_list[simp]:
-  "mset (union_mset_list l l') = mset l #\<union> mset l'"
-  by (induction l arbitrary: l') (auto simp: multiset_eq_iff)
-
-lemma "union_mset_list l [] = l"
-  by (induction l) auto
-
-interpretation cdcl\<^sub>W:  conc_state\<^sub>W_with_candidates
-  trail
-  clauses
-  learned_clss
-  backtrack_lvl conflicting
-  "\<lambda>L (M, S). (L # M, S)"
-  "\<lambda>(M, S). (tl M, S)"
-  "\<lambda>C (M, N, S). (M, {#C#} + N, S)"
-  "\<lambda>C (M, N, U, S). (M, N, {#C#} + U, S)"
-  "\<lambda>C (M, N, U, S). (M, remove_mset C N, remove_mset C U, S)"
-  "\<lambda>k (M, N, (U::nat clauses), _, D). (M, N, U, k, D)"
-  "\<lambda>D (M, N, U, k, _). (M, N, U, k, D)"
-  "\<lambda>N. ([], N, {#}, 0, None)"
-  "\<lambda>(_, N, U, _). ([], N, U, 0, None)"
-
-  trail
-  clauses
-  learned_clss
-  backtrack_lvl
-  conflicting
-  "\<lambda>L (M, S). (L # M, S)"
-  "\<lambda>(M, S). (tl M, S)"
-  "\<lambda>C (M, N, S). (M, C # N, S)"
-  "\<lambda>C (M, N, U, S). (M, N, C # U, S)"
-  "\<lambda>C (M, N, U, S). (M, removeAll C N, removeAll C U, S)"
-  "\<lambda>(k::nat) (M, N, U, _, D). (M, N, U, k, D)"
-  "\<lambda>D (M, N, U, k, _). (M, N, U, k, D)"
-  "\<lambda>N. ([], N, [], 0, None)"
-  "\<lambda>(_, N, U, _). ([], N, U, 0, None)"
-
-  "\<lambda>(M, N, U, S).
-    case find_first_unit_clause (N @ U) M of
-      None \<Rightarrow> []
-    | Some (L, a) \<Rightarrow> [(L, a)]"
-  "\<lambda>(M, N, U, S).
-    case find_conflict M (N @ U) of
-      None \<Rightarrow> []
-    | Some a \<Rightarrow> [a]"
-  "\<lambda>(M, N, U, S). find_first_unused_var (N @ U) (lits_of M)"
-  "\<lambda>(M, N, U, k, C).
-    (convert_tr M, mset (map mset N), mset (map mset U), k, map_option mset C)"
-
-  mset
-  "\<lambda>N. (map mset N)"
-  "\<lambda>a b.  (union_mset_list a b)"
-  remdups
-  convert
-  "\<lambda>C (M, N, U, k, D). maximum_level_code C M"
-  "\<lambda>S. (hd (trail S))"
-  remove1
-  apply unfold_locales
-  apply (auto simp: map_tl add.commute distinct_mset_rempdups_union_mset cdcl\<^sub>W'.clauses_def)[12]
-  apply (auto split: option.splits simp: find_conflict_None cdcl\<^sub>W'.clauses_def)[2]
-  apply (auto simp:)[]
-  using hd_map apply metis
-  apply auto[]
-
-  sorry
-
-
-definition truc :: "(nat, nat, nat literal list) marked_lit list \<times>
-   nat literal list list \<times>
-   nat literal list list \<times> nat \<times> nat literal list option
-   \<Rightarrow> ((nat, nat, nat literal list) marked_lit list \<times>
-       nat literal list list \<times>
-       nat literal list list \<times>
-       nat \<times> nat literal list option) option"
-  where
-"truc = cdcl\<^sub>W_cands.do_conflict_step  (\<lambda>(M, N, U, k, D). D) (\<lambda>C (M, N, U, k, _). (M, N, U, k, C))
-     (\<lambda>(M, N, U, S). case find_conflict M (N @ U) of None \<Rightarrow> [] | Some a \<Rightarrow> [a])"
-
-interpretation gcdcl\<^sub>W2: cdcl\<^sub>W_cands
-  trail
-  clauses
-  learned_clss
-  backtrack_lvl conflicting
-  "\<lambda>L (M, S). (L # M, S)"
-  "\<lambda>(M, S). (tl M, S)"
-  "\<lambda>C (M, N, S). (M, {#C#} + N, S)"
-  "\<lambda>C (M, N, U, S). (M, N, {#C#} + U, S)"
-  "\<lambda>C (M, N, U, S). (M, remove_mset C N, remove_mset C U, S)"
-  "\<lambda>k (M, N, (U::nat clauses), _, D). (M, N, U, k, D)"
-  "\<lambda>D (M, N, U, k, _). (M, N, U, k, D)"
-  "\<lambda>N. ([], N, {#}, 0, None)"
-  "\<lambda>(_, N, U, _). ([], N, U, 0, None)"
-
-  trail
-  clauses
-  learned_clss
-  backtrack_lvl
-  conflicting
-  "\<lambda>L (M, S). (L # M, S)"
-  "\<lambda>(M, S). (tl M, S)"
-  "\<lambda>C (M, N, S). (M, C # N, S)"
-  "\<lambda>C (M, N, U, S). (M, N, C # U, S)"
-  "\<lambda>C (M, N, U, S). (M, removeAll C N, removeAll C U, S)"
-  "\<lambda>(k::nat) (M, N, U, _, D). (M, N, U, k, D)"
-  "\<lambda>D (M, N, U, k, _). (M, N, U, k, D)"
-  "\<lambda>N. ([], N, [], 0, None)"
-  "\<lambda>(_, N, U, _). ([], N, U, 0, None)"
-
-  "\<lambda>(M, N, U, S).
-    case find_first_unit_clause (N @ U) M of
-      None \<Rightarrow> []
-    | Some (L, a) \<Rightarrow> [(L, a)]"
-  "\<lambda>(M, N, U, S).
-    case find_conflict M (N @ U) of
-      None \<Rightarrow> []
-    | Some a \<Rightarrow> [a]"
-  "\<lambda>(M, N, U, S). find_first_unused_var (N @ U) (lits_of M)"
-  "\<lambda>(M, N, U, k, C).
-    (convert_tr M, mset (map mset N), mset (map mset U), k, map_option mset C)"
-
-  mset
-  "\<lambda>N. (map mset N)"
-  "\<lambda>a b.  (union_mset_list a b)"
-  remdups
-  convert
-  "\<lambda>C (M, N, U, k, D). maximum_level_code C M"
-  "\<lambda>S. (hd (trail S))"
-  remove1
-  rewrites
-  "cdcl\<^sub>W_cands.do_conflict_step (\<lambda>(M, N, U, k, D). D) (\<lambda>C (M, N, U, k, _). (M, N, U, k, C))
-     (\<lambda>(M, N, U, S). case find_conflict M (N @ U) of None \<Rightarrow> [] | Some a \<Rightarrow> [a])
-  = truc"
-   apply unfold_locales
-   using [[show_abbrevs = false]]
-   unfolding truc_def apply simp
-  sorry
-
-
-term cdcl\<^sub>W_cands.do_conflict_step
-thm truc_def
-declare [[show_abbrevs = false, show_types = true, show_sorts]]
-thm  gcdcl\<^sub>W2.do_conflict_step_def
-declare gcdcl\<^sub>W2.do_conflict_step_def[code]
-export_code gcdcl\<^sub>W2.do_conflict_step in SML
-
+ *)
 end
